cava-examples/NandGate.v
@@ -46,11 +46,11 @@ Definition nand2Top {m t} `{CavaTop m t} :=
   c <- nand2 [a; b] ;
   output "c" c.
 
-Definition nand2Netlist := snd (nand2Top initState).
+Definition nand2Netlist := makeNetlist nand2Top.
 
 (* A proof that the NAND gate implementation is correct. *)
 Lemma nand2_behaviour : forall (a : bool) (b : bool),
-                        (fst (nand2 [a; b] tt)) = negb (a && b).
+                        combinational (nand2 [a; b]) = negb (a && b).
 Proof.
   auto.
 Qed.
